hax-lib/proof-libs/fstar/core/Alloc.Collections.Vec_deque.fsti
@@ -1,24 +1,29 @@
 module Alloc.Collections.Vec_deque
-open Rust_primitives
+#set-options "--fuel 0 --ifuel 1 --z3rlimit 15"
+open FStar.Mul
+open Core_models
 
-unfold type t_VecDeque t (_: unit) = t_Slice t
+type t_VecDeque (v_T: Type0) (v_A: Type0) =
+  | VecDeque : Rust_primitives.Seq.t_Seq v_T v_A -> t_VecDeque v_T v_A
 
-val impl_5__push_back #t #a (v: t_VecDeque t a) (x: t): t_VecDeque t a
+val impl_5__push_back (#v_T #v_A: Type0) (self: t_VecDeque v_T v_A) (x: v_T)
+    : Prims.Pure (t_VecDeque v_T v_A) Prims.l_True (fun _ -> Prims.l_True)
 
-let impl_5__len #t #a (v: t_VecDeque t a): usize = sz (Seq.length v)
+val impl_5__len (#v_T #v_A: Type0) (self: t_VecDeque v_T v_A)
+    : Prims.Pure usize Prims.l_True (fun _ -> Prims.l_True)
 
-let impl_5__pop_front #t #a (v: t_VecDeque t a): (res: t_VecDeque t a 
-  {Seq.length res == (if (Seq.length v) > 0 then (Seq.length v - 1) else Seq.length v)}) & Core_models.Option.t_Option t = 
-  match Seq.seq_to_list v with 
-  | h::tail -> Seq.seq_of_list tail,  Core_models.Option.Option_Some h 
-  | [] -> v, Core_models.Option.Option_None
+val impl_5__pop_front (#v_T #v_A: Type0) (self: t_VecDeque v_T v_A)
+    : Prims.Pure (t_VecDeque v_T v_A & Core_models.Option.t_Option v_T)
+      Prims.l_True
+      (fun _ -> Prims.l_True)
 
-
-[@FStar.Tactics.Typeclasses.tcinstance]
-val from_vec_deque_array t a n: Core_models.Convert.t_From (Alloc.Collections.Vec_deque.t_VecDeque t a)
-        (Rust_primitives.Arrays.t_Array t
-            (Rust_primitives.Integers.mk_usize n))
-
-
-val index_vec_deque t a: Core_models.Ops.Index.t_Index (Alloc.Collections.Vec_deque.t_VecDeque t a)
-        Rust_primitives.Integers.usize
+[@@ FStar.Tactics.Typeclasses.tcinstance]
+let impl_6 (#v_T #v_A: Type0) : Core_models.Ops.Index.t_Index (t_VecDeque v_T v_A) usize =
+  {
+    f_Output = v_T;
+    f_index_pre = (fun (self: t_VecDeque v_T v_A) (i: usize) -> true);
+    f_index_post = (fun (self: t_VecDeque v_T v_A) (i: usize) (out: v_T) -> true);
+    f_index
+    =
+    fun (self: t_VecDeque v_T v_A) (i: usize) -> Rust_primitives.Seq.seq_index #v_T #v_A self._0 i
+  }
