hax-lib/proof-libs/fstar/core/Rand_core.Os.fsti
@@ -1,9 +1,18 @@
 module Rand_core.Os
+#set-options "--fuel 0 --ifuel 1 --z3rlimit 15"
+open FStar.Mul
+open Rust_primitives
 
-type t_OsRng
+let _ =
+  (* This module has implicit dependencies, here we make them explicit. *)
+  (* The implicit dependencies arise from typeclasses instances. *)
+  let open Rand_core in
+  ()
 
-[@FStar.Tactics.Typeclasses.tcinstance]
-val impl_rng_core: Rand_core.t_RngCore t_OsRng
+type t_OsRng = | OsRng : t_OsRng
 
-[@FStar.Tactics.Typeclasses.tcinstance]
-val impl_crypto_rng_core: Rand_core.t_CryptoRngCore t_OsRng
+[@@ FStar.Tactics.Typeclasses.tcinstance]
+val impl:Rand_core.t_RngCore t_OsRng
+
+[@@ FStar.Tactics.Typeclasses.tcinstance]
+val impl_1:Rand_core.t_CryptoRng t_OsRng
