hax-lib/proof-libs/fstar/core/Alloc.Alloc.fst
@@ -1,3 +1,6 @@
 module Alloc.Alloc
+#set-options "--fuel 0 --ifuel 1 --z3rlimit 15"
+open FStar.Mul
+open Rust_primitives
 
-let t_Global = ()
+type t_Global = | Global : t_Global
