hax-lib/proof-libs/fstar/core/Alloc.Boxed.fst
@@ -1,5 +1,10 @@
 module Alloc.Boxed
+#set-options "--fuel 0 --ifuel 1 --z3rlimit 15"
+open FStar.Mul
+open Rust_primitives
 
-type t_Box t t_Global = t
+type t_Box (v_T: Type0) (v_A: Type0) =
+  | Box : v_T -> Core_models.Option.t_Option v_A -> t_Box v_T v_A
 
-assume val impl__new #t (v: t) : t
+let impl__new (#v_T #v_A: Type0) (v: v_T) : t_Box v_T v_A =
+  Box v (Core_models.Option.Option_None <: Core_models.Option.t_Option v_A) <: t_Box v_T v_A
